semantics/chorTypeScript.sml
@@ -1,0 +1,28 @@
+open HolKernel Parse boolLib bossLib richerLangTheory envSemTheory finite_mapTheory
+
+open chorLangTheory
+
+val _ = new_theory "chorType";
+
+
+Datatype:
+  type = typeL | unitT
+End
+
+Inductive chorTypecheck:
+[~nil:] ∀ Γ Θ. chorTypecheck Γ Θ Nil unitT
+[~com:] ∀ Γ Θ p1 v1 p2 v2 c ty. FLOOKUP Γ (v1,p1) = SOME strT ∧ ({p1,p2} ⊆ Θ) ∧
+                                chorTypecheck Γ Θ c ty ⇒
+                                chorTypecheck Γ Θ (Com p1 v1 p2 v2 c) ty
+[~sel:] ∀ Γ Θ p1 p2 b c ty. ({p1,p2} ⊆ Θ) ∧ chorTypecheck Γ Θ c ty ⇒
+                            chorTypecheck Γ Θ (Sel p1 b p2 c) ty
+[~if:] ∀ Γ Θ v p c1 c2 ty. FLOOKUP Γ (v,p) = SOME boolT ∧
+                           chorTypecheck Γ Θ c1 ty ∧ chorTypecheck Γ Θ c2 ty ⇒
+                           chorTypecheck Γ Θ (IfThen v p c1 c2) ty
+[~let:] ∀ Γ Θ v p e c ety ty. typecheck (localise Γ p) e ety ∧
+                              chorTypecheck (Γ |+ ((v,p), ety)) Θ c ty ⇒
+                              chorTypecheck Γ Θ (Let v p e c) ty
+End
+
+val _ = export_theory();
+
